not done

myex/Example_proof.thy
@@ -10,23 +10,28 @@ lemmas set_tl = list.set_sel(2)[rotated]
 lemmas Collect_conj_eq_rev = Collect_conj_eq[symmetric]
 (****************************************)
   
+definition same_target''
+  where
+    "same_target'' \<equiv> \<acute>x:=0"
+  
 definition same_target
   where
-    "same_target \<equiv> (\<acute>x:=0)"
+    "same_target \<equiv> (same_target'')"
     
 lemmas same_target_defs =
   same_target_def
   
 lemma same_target_prop_proof:
   "\<lbrace>True\<rbrace> \<parallel>-\<^sub>i \<lbrace>True\<rbrace> \<lbrace>True\<rbrace> same_target \<lbrace>True\<rbrace>"
-  unfolding same_target_defs
+  unfolding same_target_defs same_target''_def
   unfolding (*inv_defs*) oghoare_inv_def
   apply (simp add: add_inv_aux_def o_def
               del: last.simps butlast.simps)
   apply oghoare
   (*apply (find_goal \<open>succeeds \<open>rule subsetI[where A=UNIV]\<close>\<close>)*)
   (*subgoal*)
-  apply clarsimp
+  apply clarify
+    apply simp
   done
   
 end
